backend/TailcallGotoproof.v
@@ -1,0 +1,14 @@
+Require Import Coqlib Maps Integers AST Linking.
+Require Import Values Memory Events Globalenvs Smallstep.
+Require Import Op Registers RTL Conventions TailcallGoto.
+
+
+Definition match_prog (p tp: RTL.program) :=
+  match_program (fun ctx f tf => tf = transf_fundef (prog_defmap p) f) eq p tp.
+
+Lemma transf_program_match:
+  forall p, match_prog p (transf_program p).
+Proof.
+  intros. eapply match_transform_program; eauto.
+Qed.
+
